Refactor CLBT

theories/container/binary/Clbt.v
@@ -1,8 +1,38 @@
 Require Import Program Arith Lists.List.
+Require Import NumRep.utils.Utils.
 Require Import NumRep.numerical.binary.BinNat.
 Import ListNotations.
 
 Open Scope type_scope.
+
+(********************************************************************************)
+(** * Complete leaf binary tree
+
+** Constructors:
+
+- [t] == the type of leaf binary tree
+- [singleton a] == the tree made of a single element [a]
+- [create a h] == the tree of [2^h] copies of [a]
+
+** Predicates:
+
+- [is_valid h t] <=> the tree [t] is complete of height [h]
+
+All the constructors exposed in this module produce valid binary trees
+while operations preserve validity.
+
+** Operations:
+
+- [card t] == number of elements (ie., leafs) in [t]
+- [merge l r] == merge two valid trees [l] and [r] of height [h] into
+  a valid tree of height [h+1]
+- [lookup t dn] == lookup the [dn]-th leaf (counted from left to right)
+  of [t], with [dn] in MSB-first form
+- [update t dn a] == update the [dn]-th element of [t] with [a]
+
+*)
+(********************************************************************************)
+
 
 Section CLBT.
 
@@ -12,26 +42,25 @@ Inductive t :=
 	| Leaf : A -> t
 	| Node : t -> t -> t.
 
+(** [is_valid] *)
+
 Inductive is_valid : nat -> t -> Prop :=
 	| valid_Leaf : forall a : A, is_valid 0 (Leaf a)
 	| valid_Node : forall {n : nat} (l r : t),
 		is_valid n l -> is_valid n r ->
 		is_valid (S n) (Node l r).
 
-Definition singleton (a : A) : t := Leaf a.
-Lemma singleton_valid : forall a : A, is_valid 0 (singleton a).
-Proof.
-	intro a.
-	apply valid_Leaf.
-Qed.
+Hint Constructors is_valid : core.
 
-Fixpoint size t : nat :=
+(** [card] *)
+
+Fixpoint card t : nat :=
 	match t with
 	| Leaf _ => 1
-	| Node l r => size l + size r
+	| Node l r => card l + card r
 	end.
 
-Lemma valid_size : forall n t, is_valid n t -> size t = 2 ^ n.
+Lemma valid_card : forall n t, is_valid n t -> card t = 2 ^ n.
 Proof.
 	intros n t H.
 	{	induction H as [|n l r _ HRl _ HRr].
@@ -42,283 +71,125 @@ Proof.
 	}
 Qed.
 
+(** [create] *)
+
+Fixpoint create (a : A)(h: nat) : t := 
+  match h with
+  | O => Leaf a
+  | S n => let t := create a n in Node t t
+  end.
+
+Lemma create_valid : forall a h, is_valid h (create a h).
+Proof. intros ? h; induction h; simpl; auto. Qed.
+
+(** [singleton] *)
+
+Definition singleton (a : A) : t := create a 0.
+
+Lemma singleton_valid : forall a, is_valid 0 (singleton a).
+Proof. auto using create_valid. Qed.
+
+(** [merge l r] *)
+
 Definition merge (l r : t) : t := Node l r.
 Lemma merge_valid : forall {n : nat} (l r : t),
 	is_valid n l -> is_valid n r -> is_valid (S n) (merge l r).
-Proof.
-	intros n l r Hl Hr.
-	apply valid_Node; assumption.
-Qed.
+Proof. intros *; auto using valid_Node. Qed.
 
-Fixpoint head t : A :=
-	match t with
-	| Leaf a => a
-	| Node _ r => head r
-	end.
-
-Definition left t :=
-	match t with
-	| Leaf _ => t
-	| Node l _ => l
-	end.
-Definition right t :=
-	match t with
-	| Leaf _ => t
-	| Node _ r => r
-	end.
-
-Lemma left_valid : forall {n : nat} t,
-	is_valid (S n) t -> is_valid n (left t).
-Proof.
-	intros n t H.
-	inversion_clear H.
-	assumption.
-Qed.
-
-Lemma right_valid : forall {n : nat} t,
-	is_valid (S n) t -> is_valid n (right t).
-Proof.
-	intros n t H.
-	inversion_clear H.
-	assumption.
-Qed.
-
-Fixpoint update t dn a :=
-	match t, dn with
-	| Leaf _, [] => Leaf a
-	| Node l r, 0 :: tdn => Node l (update r tdn a)
-	| Node l r, 1 :: tdn => Node (update l tdn a) r
-	| _, _ => t
-	end.
+(** [lookup] *)
 
 Fixpoint lookup t dn :=
 	match t, dn with
-	| Leaf a, _ => a
-	| _, [] => head t
-	| Node _ r, 0 :: tdn => lookup r tdn
-	| Node l _, 1 :: tdn => lookup l tdn
+	| Leaf a, [] => Some a
+	| Node l _, 0 :: tdn => lookup l tdn
+	| Node _ r, 1 :: tdn => lookup r tdn
+        | _, _ => (* Impossible *) None
 	end.
+
+(** [update] *)
+
+
+Fixpoint update t dn a :=
+	match t, dn with
+	| Leaf _, [] => Some (Leaf a)
+	| Node l r, 0 :: tdn => option_map (fun l => Node l r) (update l tdn a)
+	| Node l r, 1 :: tdn => option_map (fun r => Node l r) (update r tdn a)
+	| _, _ => None
+	end.
+
+Definition is_valid_idx (n: list Bit) t: Prop :=
+  is_valid (length n) t.
+
+Hint Unfold is_valid_idx : core.
 
 Lemma update_valid : forall n t a,
-		is_valid (length n) t ->
-		is_valid (length n) (update t n a).
+		is_valid_idx n t ->
+		option_lift (fun t => is_valid_idx n t) (update t n a).
 Proof.
 	intro n.
-	{	induction n as [|bn tn HR]; [|destruct bn]; simpl;
-			intros t a Ht; inversion_clear Ht; simpl.
-	+	apply valid_Leaf.
-	+	apply (HR _ a) in H0.
-		apply valid_Node; assumption.
-	+	apply (HR _ a) in H.
-		apply valid_Node; assumption.
-	}
+        {
+	  induction n as [|[ | ] tn IH];
+            intros t a Ht;
+            inversion_clear Ht as [|? l r Hl Hr];
+            simpl.
+          1: apply valid_Leaf.
+          all:
+	    rewrite lift_map; simpl;
+            eapply lift_conseq
+              with (P := is_valid_idx tn); auto;
+            intros; eauto using valid_Node.
+        }
 Qed.
+
+Lemma update_total: forall n t a,
+    is_valid_idx n t ->
+    exists t', update t n a = Some t'.
+Proof.
+  intro n.
+  {
+    induction n as [| [|] tn IH];
+      intros t a Ht;
+      inversion_clear Ht as [|? l r Hl Hr];
+      simpl; eauto.
+    all: edestruct IH as [? ->]; eauto;
+      simpl; eauto.
+  }
+Qed.
+
+(** Equational theory [update]/[lookup] *)
 
 Lemma lookup_update_eq : forall n t a,
-		is_valid (length n) t ->
-		lookup (update t n a) n = a.
+		is_valid_idx n t ->
+		option_bind (update t n a) (fun t => lookup t n) = Some a.
 Proof.
 	intro n.
-	{	induction n as [|bn tn HR]; [|destruct bn]; simpl;
-			intros t a Ht; inversion_clear Ht; simpl.
-	+	reflexivity.
-	+	apply HR.
-		assumption.
-	+	apply HR.
-		assumption.
-	}
+	{
+          induction n as [|[|] tn IH];
+	    intros t a Ht;
+            inversion_clear Ht as [|? l r Hl Hr];
+            simpl; auto.
+          all: rewrite bind_map; eauto.
+        }
 Qed.
+
 Lemma lookup_update_neq : forall n m t a,
-		(length n) = (length m) -> n <> m ->
-		is_valid (length n) t ->
-		lookup (update t n a) m = lookup t m.
+		length n = length m -> n <> m ->
+		is_valid_idx n t ->
+		option_bind (update t n a) (fun t => lookup t m) = lookup t m.
 Proof.
 	intro n.
-	{	induction n as [|bn tn HR]; [|destruct bn];	intros m t a Hlen Hneq Ht;
-			(destruct m as [|bm tm]; [|destruct bm]); simpl;
-			inversion_clear Ht; simpl in *.
-	+	contradiction.
-	+	discriminate.
-	+	discriminate.
-	+	discriminate.
-	+	apply eq_add_S in Hlen.
-		assert (tn <> tm) by (intro Ha; rewrite Ha in Hneq; apply Hneq; reflexivity).
-		apply HR; assumption.
-	+	reflexivity.
-	+	reflexivity.
-	+	reflexivity.
-	+	apply eq_add_S in Hlen.
-		assert (tn <> tm) by (intro Ha; rewrite Ha in Hneq; apply Hneq; reflexivity).
-		apply HR; assumption.
-	}
-Qed.
-
-Inductive dt :=
-	| DRoot : dt
-	| DLeft : dt -> t -> dt
-	| DRight : t -> dt -> dt.
-
-Inductive is_valid_d : nat -> nat -> dt -> Prop :=
-	| valid_DRoot : forall (n : nat), is_valid_d n n DRoot
-	| valid_DLeft : forall (d n : nat) dt t,
-		is_valid_d d (S n) dt -> is_valid n t ->
-		is_valid_d d n (DLeft dt t)
-	| valid_DRight : forall (d n : nat) dt t,
-		is_valid n t -> is_valid_d d (S n) dt ->
-		is_valid_d d n (DRight t dt).
-
-Definition zip := t * dt.
-Definition make_zip t : zip := (t, DRoot).
-
-Definition is_valid_zip (d n : nat) zip :=
-	is_valid n (fst zip) /\ is_valid_d d n (snd zip).
-
-Lemma make_zip_valid : forall t n,
-		is_valid n t -> is_valid_zip n n (make_zip t).
-Proof.
-	intros t n H.
-	split; [assumption| apply valid_DRoot].
-Qed.
-
-
-Fixpoint dtrace dt :=
-	match dt with
-	| DRoot => []
-	| DLeft dt _ => 1 :: (dtrace dt)
-	| DRight _ dt => 0 :: (dtrace dt)
-	end.
-
-Definition down_left '(t, dt) :=
-	match t with
-	| Leaf _ => (t, dt)
-	| Node l r => (l, DLeft dt r)
-	end.
-
-Lemma down_left_valid : forall zip {d n : nat},
-	is_valid_zip d (S n) zip -> is_valid_zip d n (down_left zip).
-Proof.
-	intros zip d n H.
-	destruct zip as [t dt].
-	destruct H as [Ht Hdt]; simpl in *.
-	inversion_clear Ht.
-	{	split.
-	+	assumption.
-	+	apply valid_DLeft; assumption.
-	}
-Qed.
-
-Definition down_right '(t, dt) :=
-	match t with
-	| Leaf _ => (t, dt)
-	| Node l r => (r, DRight l dt)
-	end.
-
-Lemma down_right_valid : forall zip {d n : nat},
-	is_valid_zip d (S n) zip -> is_valid_zip d n (down_right zip).
-Proof.
-	intros zip d n H.
-	destruct zip as [t dt].
-	destruct H as [Ht Hdt]; simpl in *.
-	inversion_clear Ht.
-	{	split.
-	+	assumption.
-	+	apply valid_DRight; assumption.
-	}
-Qed.
-
-Definition up '(t, dt) :=
-	match dt with
-	| DRoot => (t, dt)
-	| DLeft dt r => (Node t r, dt)
-	| DRight l dt => (Node l t, dt)
-	end.
-
-Fixpoint plug t dt :=
-	match dt with
-	| DRoot => t
-	| DLeft dt r => plug (Node t r) dt
-	| DRight l dt => plug (Node l t) dt
-	end.
-
-Lemma plug_valid : forall dt t n d,
-		is_valid d t -> is_valid_d n d dt ->
-		is_valid n (plug t dt).
-Proof.
-	intro dt.
-	{	induction dt as [| dt HR r | l dt HR]; intros t n d Ht Hdt;
-			inversion_clear Hdt; simpl in *.
-	+	assumption.
-	+	apply (HR _ _ (S d)); [|assumption].
-		apply valid_Node; assumption.
-	+	apply (HR _ _ (S d)); [|assumption].
-		apply valid_Node; assumption.
-	}
-Qed.
-
-Fixpoint open zip dn :=
-	match dn with
-	| [] => zip
-	| 0 :: tdn => open (down_right zip) tdn
-	| 1 :: tdn => open (down_left zip) tdn
-	end.
-
-Lemma open_lookup : forall t dn,
-		is_valid (length dn) t ->
-		fst (open (make_zip t) dn) = Leaf (lookup t dn).
-Proof.
-	enough (H : forall t dt dn, is_valid (length dn) t ->
-						   fst (open (t, dt) dn) = Leaf (lookup t dn))
-		by (intros t dn; apply H).
-	intro t.
-	{	induction t as [t|l HRl r HRr]; intros dt dn H.
-	+	inversion H as [t' Hl Ht'|].
-		apply eq_sym, length_zero_iff_nil in Hl.
-		rewrite Hl.
-		reflexivity.
-	+	destruct dn as [|bn tn]; inversion_clear H.
-		destruct bn; [apply HRr|apply HRl]; assumption.
-	}
-Qed.
-
-Lemma open_valid : forall dn zip d,
-		is_valid_zip d (length dn) zip ->
-		is_valid_zip d 0 (open zip dn).
-Proof.
-	intro dn.
-	{	induction dn as [|b tdn HR]; intros zip d H; [|destruct b]; simpl.
-	+	assumption.
-	+	apply HR.
-		apply down_right_valid.
-		assumption.
-	+	apply HR.
-		apply down_left_valid.
-		assumption.
-	}
-Qed.
-
-Lemma open_trace : forall dn d n zip,
-		is_valid_zip d n zip -> (length dn) <= n ->
-		dtrace (snd (open zip dn)) = rev_append dn (dtrace (snd zip)).
-Proof.
-	intro dn.
-	{	induction dn as [|b tn HR]; intros d n zip Hz Hdn; [|destruct b]; simpl in *.
-	+	reflexivity.
-	+	destruct n; [apply Nat.nle_succ_0 in Hdn; contradiction|].
-		apply down_right_valid in Hz as He.
-		apply HR in He; [|apply le_S_n; assumption].
-		rewrite He.
-		unfold down_right.
-		destruct zip as [t dt], Hz as [Ht Hdt]; simpl in *.
-		inversion_clear Ht.
-		reflexivity.
-	+	destruct n; [apply Nat.nle_succ_0 in Hdn; contradiction|].
-		apply down_left_valid in Hz as He.
-		apply HR in He; [|apply le_S_n; assumption].
-		rewrite He.
-		unfold down_right.
-		destruct zip as [t dt], Hz as [Ht Hdt]; simpl in *.
-		inversion_clear Ht.
-		reflexivity.
+	{
+          induction n as [|[|] tn IH];
+            intros [|[|] tm] t a Hlen Hneq Ht;
+            inversion_clear Ht;
+            simpl in *;
+            try tauto;
+            rewrite bind_map; simpl;
+            try solve [
+                rewrite bind_fail; auto
+              | eapply IH; auto;
+                congruence 
+              | edestruct update_total as [? ->]; auto ].
 	}
 Qed.
 
